thys/JinjaThreads/MM/SC.thy
@@ -428,4 +428,12 @@ code_pred
   (modes: i \<Rightarrow> i \<Rightarrow> i \<Rightarrow> i \<Rightarrow> i \<Rightarrow> bool, i \<Rightarrow> i \<Rightarrow> i \<Rightarrow> i \<Rightarrow> o \<Rightarrow> bool)
   sc_heap_write .
 
+lemma eval_sc_heap_read_i_i_i_o:
+  "Predicate.eval (sc_heap_read_i_i_i_o h ad al) = sc_heap_read h ad al"
+by(auto elim: sc_heap_read_i_i_i_oE intro: sc_heap_read_i_i_i_oI intro!: ext)
+
+lemma eval_sc_heap_write_i_i_i_i_o:
+  "Predicate.eval (sc_heap_write_i_i_i_i_o h ad al v) = sc_heap_write h ad al v"
+by(auto elim: sc_heap_write_i_i_i_i_oE intro: sc_heap_write_i_i_i_i_oI intro!: ext)
+
 end
